Add select

src/Experiments/NewPipeline/Arithmetic.v
@@ -490,32 +490,58 @@ Module Positional. Section Positional.
   Hint Rewrite @length_sub @length_opp : distr_length.
 
   Section select.
-    Definition select (mask cond:Z) (p:list Z) :=
+    Definition zselect (mask cond:Z) (p:list Z) :=
       dlet t := Z.zselect cond 0 mask in List.map (Z.land t) p.
+
+    Definition select (cond:Z) (if_zero if_nonzero:list Z) :=
+      List.map (fun '(p, q) => Z.zselect cond p q) (List.combine if_zero if_nonzero).
 
     Lemma map_and_0 n (p:list Z) : length p = n -> map (Z.land 0) p = zeros n.
     Proof.
       intro; subst; induction p as [|x xs IHxs]; [reflexivity | ].
       cbn; f_equal; auto.
     Qed.
-    Lemma eval_select n mask cond p (H:List.map (Z.land mask) p = p) :
+    Lemma eval_zselect n mask cond p (H:List.map (Z.land mask) p = p) :
       length p = n
-      -> eval n (select mask cond p) =
+      -> eval n (zselect mask cond p) =
          if dec (cond = 0) then 0 else eval n p.
     Proof.
-      cbv [select Let_In].
+      cbv [zselect Let_In].
       rewrite Z.zselect_correct; break_match.
       { intros; erewrite map_and_0 by eassumption. apply eval_zeros. }
       { rewrite H; reflexivity. }
     Qed.
-    Lemma length_select mask cond p :
-      length (select mask cond p) = length p.
-    Proof using Type. clear dependent weight. cbv [select Let_In]; break_match; intros; distr_length. Qed.
+    Lemma length_zselect mask cond p :
+      length (zselect mask cond p) = length p.
+    Proof using Type. clear dependent weight. cbv [zselect Let_In]; break_match; intros; distr_length. Qed.
+    Lemma eval_select n cond p q :
+      length p = n -> length q = n
+      -> eval n (select cond p q) =
+         if dec (cond = 0) then eval n p else eval n q.
+    Proof.
+      cbv [select Let_In]; intro; subst.
+      rewrite <- (List.rev_involutive q), <- (List.rev_involutive p).
+      generalize (rev p) (rev q); clear p q; intros p q; revert q.
+      induction p as [|p ps IHps], q as [|q qs]; cbn [length map combine rev]; distr_length; rewrite ?Nat.add_1_r; try omega.
+      { break_match; reflexivity. }
+      { intro; rewrite !combine_snoc, !map_app by (distr_length; omega).
+        cbn [map].
+        rewrite !eval_snoc with (n:=length ps), IHps by (distr_length; omega* ).
+        rewrite !Z.zselect_correct; break_match; reflexivity. }
+    Qed.
+    Lemma length_select_min cond p q :
+      length (select cond p q) = Nat.min (length p) (length q).
+    Proof using Type. clear dependent weight. cbv [select Let_In]; distr_length. Qed.
+    Hint Rewrite length_select_min : distr_length.
+    Lemma length_select n cond p q :
+      length p = n -> length q = n ->
+      length (select cond p q) = n.
+    Proof using Type. clear dependent weight. distr_length; omega **. Qed.
   End select.
 End Positional.
 (* Hint Rewrite disappears after the end of a section *)
-Hint Rewrite length_zeros length_add_to_nth length_from_associational @length_add @length_carry_reduce @length_chained_carries @length_encode @length_sub @length_opp @length_select : distr_length.
-Hint Rewrite @eval_select : push_eval.
+Hint Rewrite length_zeros length_add_to_nth length_from_associational @length_add @length_carry_reduce @length_chained_carries @length_encode @length_sub @length_opp @length_select @length_zselect @length_select_min : distr_length.
+Hint Rewrite @eval_select @eval_zselect : push_eval.
 Section Positional_nonuniform.
   Context (weight weight' : nat -> Z).
 
@@ -1759,6 +1785,7 @@ Module Rows.
         fst (flatten n inp) = partition n (eval n inp).
       Proof using wprops. auto using nth_default_partitions, flatten_partitions, length_flatten. Qed.
     End Flatten.
+    Hint Rewrite length_partition : distr_length.
 
     Section Ops.
       Definition add n p q := flatten n [p; q].
@@ -1773,8 +1800,13 @@ Module Rows.
       Definition sub n p q := flatten n [p; map (fun x => dlet y := x in Z.opp y) q].
 
       Definition conditional_add n mask cond (p q:list Z) :=
-        let qq := Positional.select mask cond q in
+        let qq := Positional.zselect mask cond q in
         add n p qq.
+
+      (* Subtract q if and only if p >= q. *)
+      Definition conditional_sub n (p q:list Z) :=
+        let '(v, c) := sub n p q in
+        Positional.select c v p.
 
       Hint Rewrite eval_cons eval_nil using solve [auto] : push_eval.
 
@@ -1863,6 +1895,11 @@ Module Rows.
         base <> 0 -> n <> 0%nat -> m <> 0%nat -> length p = n -> length q = n ->
         fst (mul base n m p q) = partition m (Positional.eval weight n p * Positional.eval weight n q).
       Proof using wprops. solver. Qed.
+
+      Lemma length_mul base n m p q :
+        length p = n -> length q = n ->
+        length (fst (mul base n m p q)) = m.
+      Proof using wprops. solver; distr_length. Qed.
 
       Lemma eval_sat_reduce base s c p :
         base <> 0 -> s - Associational.eval c <> 0 -> s <> 0 ->
